bigstep typechecks

core_c_trivial_bigstep.v
@@ -1,5 +1,10 @@
 Require Export ZArith.
 Require Export ch2o.core_c.expressions.
+Require Export ch2o.memory_separation.memory_singleton.
+Require Export ch2o.separation.permissions.
+Require Export ch2o.core_c.expressions.
+Require Export ch2o.core_c.expression_eval.
+Require Export ch2o.core_c.restricted_smallstep.
 
 Notation store := (list (option Z)).
 
@@ -7,15 +12,15 @@ Inductive mem_stack `{Env K} (Γ : env K) (Δ : memenv K): stack K -> store -> m
 | mem_stack_empty m:
   mem_stack Γ Δ [] [] m
 | mem_stack_alloc o mv m ρ st m':
-  mem_singleton Γ Δ (addr_top o sintT%T) false full_perm
-    (match mv with None => indetV sintT%T | Some z => intV{sintT} z end)
+  mem_singleton Γ Δ (addr_top o sintT%T) false perm_full
+    (match mv with None => indetV sintT%BT | Some z => intV{sintT} z end)
     sintT%T m ->
   mem_stack Γ Δ ρ st m' ->
   m ⊥ m' ->
   mem_stack Γ Δ ((o, sintT%T)::ρ) (mv::st) (m ∪ m')
 .
 
-Inductive eval: store -> expr -> Z -> Prop :=
+Inductive eval `{Env K}: store -> expr K -> Z -> Prop :=
 | eval_lit st z:
   eval st (# intV{sintT} z) z
 | eval_var st i z:
@@ -23,52 +28,55 @@ Inductive eval: store -> expr -> Z -> Prop :=
   eval st (load (var i)) z
 .
 
-Lemma eval_sound:
+Lemma eval_sound `{Env K} (Γ: env K) st e z ρ m:
   eval st e z ->
-  mem_stack ρ st m ->
-  ⟦ e ⟧ Γ ρ m = Some (# intV{sintT} z).
-  
+  mem_stack Γ '{m} ρ st m ->
+  ⟦ e ⟧ Γ ρ m = Some (inr (intV{sintT} z)).
+Admitted.
+
 Inductive outcome := onormal(s: store) | oreturn(z: Z).
 
-Inductive exec: store -> stmt -> outcome -> Prop :=
-| exec_local st s:
+Inductive exec `{Env K}: store -> stmt K -> outcome -> Prop :=
+| exec_local st s O:
   exec (None::st) s O ->
   exec st (local{sintT%BT} s) O
 | exec_assign st i e z:
   eval st e z ->
-  exec st (var i ::= cast{sintT%BT} e) (onormal (<i:=Some z>st))
+  exec st (var i ::= cast{sintT%BT} e) (onormal (<[i:=Some z]>st))
 | exec_seq st s1 st' s2 O:
   exec st s1 (onormal st') ->
   exec st s2 O ->
   exec st (s1 ;; s2) O
-| exec_ret st e:
+| exec_ret st e z:
   eval st e z ->
   exec st (ret (cast{sintT%BT} e)) (oreturn z)
 .
 
-Definition is_final_state S := forall Γ δ S', ~ Γ\ δ\ [] ⊢ₛ S ⇒ S'.
+Definition is_final_state `{Env K} S := forall Γ δ S', ~ Γ\ δ\ [] ⊢ₛ S ⇒ S'.
 
-Lemma bigstep_sound_lemma st s O (P: Prop):
+Lemma bigstep_sound_lemma `{Env K} st s O (P: Prop):
   exec st s O ->
   forall Γ δ k m S,
   is_final_state S ->
   Γ\ δ\ [] ⊢ₛ State k (Stmt ↘ s) m ⇒* S ->
-  mem_stack (rlocals [] k) st m ->
+  mem_stack Γ '{m} (rlocals [] k) st m ->
   (forall st' m',
    O = onormal st' ->
-   mem_stack (rlocals [] k) st' m' ->
+   mem_stack Γ '{m'} (rlocals [] k) st' m' ->
    Γ\ δ\ [] ⊢ₛ State k (Stmt ↗ s) m' ⇒* S ->
    P) ->
   (forall z st' m',
-   O = oret z ->
-   mem_stack (rlocals [] k) st' m' ->
+   O = oreturn z ->
+   mem_stack Γ '{m'} (rlocals [] k) st' m' ->
    Γ\ δ\ [] ⊢ₛ State k (Stmt (⇈ intV{sintT} z) s) m' ⇒* S ->
    P) ->
   P.
+Admitted.
 
-Theorem bigstep_sound s z:
+Theorem bigstep_sound `{Env K} s z:
   exec [] s (oreturn z) ->
   forall Γ δ S,
   Γ\ δ\ [] ⊢ₛ State [] (Stmt ↘ s) ∅ ⇒* S ->
   exists m,
-  Γ\ δ\ [] ⊢ₛ S ⇒* State [] (Stmt ⇈ (intV{sintT} z) s) m.
+  Γ\ δ\ [] ⊢ₛ S ⇒* State [] (Stmt (⇈ (intV{sintT} z)) s) m.
+Admitted.
